\documentclass[12pt,a4paper]{report}
\usepackage[utf8]{inputenc}
\usepackage{amsmath}
\usepackage{amsfonts}
\usepackage{amssymb}
\author{Frederik Appel Vardinghus-Nielsen}
\begin{document}
\noindent{\Huge 5 Two random variables -- conditional expectation}\\\\
\begin{itemize}
\setlength\itemsep{0em}
\item Define conditional expectation
\item Prove Law of Total Expectation
\item $E[Y]=E[E[Y|X]]$
\item $\text{Var}[Y|X]=E[Y^2|X]-(E[Y|X])^2$
\item Prove special variance
\end{itemize}
\textbf{Definition 3.12.} Suppose $X$ and $Y$ are jointly continuous. We define
\begin{equation}
E[Y|X=x]=\int_{-\infty}^{\infty}\!yf_Y(y|x)\,dy
\end{equation}
\textbf{Proposition 3.6} Let $X$ and $Y$ be jointly continuous. Then
\begin{equation}
f_Y=\int_{-\infty}^{\infty}\!f_Y(y|x|)f_X(x)\,dx
\end{equation}
\textbf{Proposition 3.17. (Law of Total Expectation)} Suppose that $X$ and $Y$ are jointly continuous. Then
\begin{equation}
E[Y]=\int_{-\infty}^{\infty}E[Y|X=x]f_X(x)\,dx
\end{equation}
\textbf{Bevis}\\
By definition of expected value and proposition 3.6
\begin{equation}
E[Y]=\int_{-\infty}^{\infty}\!yf_Y(y)\,dy=\int_{-\infty}^{\infty}\!yf_Y(y|x)f_X(x)\,dx
\end{equation}
Change order of integration
\begin{equation}
E[Y]=\int_{-\infty}^{\infty}\!\int_{-\infty}^{\infty}\!yf_Y(y|x)\,dyf_X(x)\,dx
\end{equation}
The inner integral is the definition of $E[Y|X=x]$.\\\\
\textbf{Corollary 3.5.}
\begin{equation}
E[Y]=E\left[E[Y|X]\right]
\end{equation}
\textbf{Corollary 3.7.}
\begin{equation}
\text{Var}[Y|X]=E[Y^2|X]-(E[Y|X])^2
\end{equation}
\textbf{Proposition 3.19.}
\begin{equation}
\text{Var}[Y]=\text{Var}[E[Y|X]]+E[\text{Var}[Y|X]]
\end{equation}
\textbf{Bevis}\\
Take the expected value on corollary 3.7:
\begin{align*}
E[\text{Var}[Y|X]]&=E[E[Y^2|X]]-E[(E[Y|X])^2]\\
&=E[Y^2]-E[(E[Y|X])^2]
\end{align*}
Use the fact, that
\begin{equation}
\text{Var}[X]=E[X^2]-(E[X])^2
\end{equation}
and corollary 3.5 to write
\begin{align*}
\text{Var}[E[Y|X]]&=E[(E[Y|X)^2]-(E[E[Y|X])^2\\
&=E[(E[Y|X])^2]-(E[Y])^2
\end{align*}
Add the two equations:
\begin{align*}
E[\text{Var}[Y|X]]+\text{Var}[E[Y|X]]&=E[Y^2]-E[(E[Y|X])^2]+E[(E[Y|X])^2]-(E[Y])^2\\
&=E[Y^2]-(E[Y])^2\\
&=\text{Var}[Y]
\end{align*}
Gør opmærksom på hvor vigtigt resultatet er.



















\end{document}